work in progress useimmediate examples

compiler/src/compiler/UseImmediateDef.v
@@ -1,4 +1,6 @@
 Require Import compiler.util.Common.
+Require Import compiler.FlattenExprDef. (* Only imported for testing UseImmediate *)
+Require Import compiler.StringNameGen. (* Only imported for testing UseImmediate *)
 Require Import compiler.FlatImp.
 Require Import Coq.Lists.List. Import ListNotations.
 Require Import bedrock2.Syntax.
@@ -7,80 +9,154 @@ Require Import String.
  
 Open Scope Z_scope.
 
-Print stmt.
-Print exec.
-Print operand.
+Definition ex0 := (["a"], [] : list string, Syntax.cmd.set "a" (Syntax.expr.op bopname.add (Syntax.expr.literal 1) (Syntax.expr.literal 2))).
+Definition ex1 := (["b"], ["a"], Syntax.cmd.set "b" (Syntax.expr.op bopname.add (Syntax.expr.var "a") (Syntax.expr.literal 1))).
+Definition ex2 := (["b"], ["a"], Syntax.cmd.set "b" (Syntax.expr.op bopname.add (Syntax.expr.literal 1) (Syntax.expr.var "a"))).
+Definition ex3 := (["c"], ["a"], Syntax.cmd.stackalloc "b" 4
+                                              (Syntax.cmd.seq
+                                                 (Syntax.cmd.set "b"
+                                                    (Syntax.expr.op bopname.mul
+                                                       (Syntax.expr.literal 1)
+                                                       (Syntax.expr.op bopname.add
+                                                          (Syntax.expr.var "a")
+                                                          (Syntax.expr.literal 2))))
+                                                 (Syntax.cmd.set "c"
+                                                    (Syntax.expr.op bopname.add
+                                                       (Syntax.expr.literal 0)
+                                                       (Syntax.expr.op bopname.mul
+                                                          (Syntax.expr.literal 3)
+                                                          (Syntax.expr.var "b")))))).
+                                                          
+                                                    
+                                                                                       
 
-Definition literalFitsInBits(signed: bool)(bitwidth: Z)(lit: Z): bool :=
-  match signed with
-  | true =>  (- (Z.pow 2 (bitwidth - 1)) <=? lit) && (lit <? (Z.pow 2 (bitwidth - 1)))
-  | false => (0 <? lit) && (lit <? (Z.pow 2 bitwidth))
+Definition sourceExs := [ex0; ex1; ex2; ex3].
+Definition unwrappedFlattenExs := let tmp :=  List.all_success (map flatten_function sourceExs) in
+                                  match tmp with
+                                  | Success l => l
+                                  | _ => []
+                                  end.
+Compute unwrappedFlattenExs.
+(* Fixpoint list_len {A: Type} (l: list A) : nat :=
+  match l with
+  | hd :: tl => 1 + list_len tl
+  | _ => 0
   end.
 
-Fixpoint useImmediate(s: stmt string) : stmt string :=
-  match s with               
-  | SSeq s12 s3 => let default := SSeq (useImmediate s12) (useImmediate s3)
-                   in
-                   match s12, s3 with
-                   | SSeq s1 s2, SOp v3 op v1' (Var v2') => match op with
-                                                            | Syntax.bopname.add
-                                                            | Syntax.bopname.and
-                                                            | Syntax.bopname.or
-                                                            | Syntax.bopname.xor => match s1, s2 with
-                                                                                    | SLit v1 l1, SLit v2 l2 =>
-                                                                                        (*maybe stronger optimization, given both literals known? *)
-                                                                                        if andb (eqb v2 v2') (literalFitsInBits true 12 l2)
-                                                                                        then
-                                                                                          SSeq s1 (SOp v3 op v1' (Const l2))
-                                                                                        else
-                                                                                          if andb (eqb v1 v1') (literalFitsInBits true 12 l1)
-                                                                                          then
-                                                                                            SSeq s2 (SOp v3 op v2' (Const l1))
-                                                                                          else default
-                                                                                        
-                                                                                    | SLit v1 l1, _ => if andb (eqb v1 v1') (literalFitsInBits true 12 l1)
-                                                                                                       then
-                                                                                                         SSeq s2 (SOp v3 op v2' (Const l1))
-                                                                                                       else
-                                                                                                         default
-                                                                                    | _, SLit v2 l2 => if andb (eqb v2 v2') (literalFitsInBits true 12 l2) 
-                                                                                                       then
-                                                                                                         SSeq s1 (SOp v3 op v1' (Const l2))
-                                                                                                       else
-                                                                                                         default
-                                                                                    | _, _ => default
-                                                                                    end
-                                                            | Syntax.bopname.ltu
-                                                            | Syntax.bopname.lts => match s2 with
-                                                                                    | SLit v2 l2 => if andb (eqb v2 v2') (literalFitsInBits true 12 l2) 
-                                                                                                       then
-                                                                                                         SSeq s1 (SOp v3 op v1' (Const l2))
-                                                                                                       else
-                                                                                                         default
-                                                                                    | _ => default
-                                                                                    end
-                                                            | Syntax.bopname.srs
-                                                            | Syntax.bopname.slu
-                                                            | Syntax.bopname.sru => match s2 with
-                                                                                    | SLit v2 l2 => if andb (eqb v2 v2') (literalFitsInBits false 5 l2) 
-                                                                                                       then
-                                                                                                         SSeq s1 (SOp v3 op v1' (Const l2))
-                                                                                                       else
-                                                                                                         default
-                                                                                    | _ => default
-                                                                                    end
-                                                            | Syntax.bopname.sub => match s2 with
-                                                                                    | SLit v2 l2 => if andb (eqb v2 v2') (literalFitsInBits true 12 (-l2)) 
-                                                                                                       then
-                                                                                                         SSeq s1 (SOp v3 Syntax.bopname.add v1' (Const (-l2)))
-                                                                                                       else
-                                                                                                         default
-                                                                                    | _ => default
-                                                                                    end
-                                                            | _ => default
-                                                            end 
-                   | _, _ =>  default
+Compute list_len sourceExs.
+Compute list_len unwrappedFlattenExs.*)
+(*
+Definition unsignedFitsBits(bitwidth: Z)(lit: Z): bool := (0 <=? lit) && (lit <? Z.pow 2 bitwidth).
+Definition signedFitsBits(bitwidth: Z)(lit: Z): bool := (- (Z.pow 2 (bitwidth - 1)) <=? lit) && (lit <? (Z.pow 2 (bitwidth - 1))).
+*)
+Section WithArgs.
+  Context (is5BitImmediate : Z -> bool).
+  Context (is12BitImmediate: Z -> bool).
+
+  
+  
+  Fixpoint useImmediate(s: stmt string) : stmt string :=
+    match s with
+    | SIf c s1 s2 => SIf c (useImmediate s1) (useImmediate s2)
+    | SLoop s1 c s2 => SLoop (useImmediate s1) c (useImmediate s2)
+    | SStackalloc v1 sz1 s => SStackalloc v1 sz1 (useImmediate s)
+    | SSeq s1 s2 =>
+        let used1 := useImmediate s1 in
+        let used2 := useImmediate s2 in
+        let default := SSeq used1 used2 in
+        match used1, used2 with
+        | SSkip, _ => used2
+        | _, SSkip => used1
+        | SLit v1 l1, SOp v2 op v2a (Var v2b) => default
+        | SLit v1 l1, SSeq (SLit v1b l1b) (SOp v2 op v2a (Var v2b)) =>
+            if (eqb v1 v1b) then default else default
+        | _, _ => default
+        end
+    | _ => s
+    end.
+  (*
+  Fixpoint useImmediate(s: stmt string) : stmt string :=
+    match s with               
+    | SSeq s12 s3 =>
+        let default := SSeq (useImmediate s12) (useImmediate s3)
+        in match s12, s3 with
+           | SSeq s1 s2, SOp v3 op v1' (Var v2') =>
+               match op with
+               | Syntax.bopname.add
+               | Syntax.bopname.and
+               | Syntax.bopname.or
+               | Syntax.bopname.xor =>
+                   match s1, s2 with
+                   | SLit v1 l1, SLit v2 l2 =>
+                       if andb (eqb v2 v2') (is12BitImmediate l2)
+                       then SSeq s1 (SOp v3 op v1' (Const l2))
+                       else
+                         if andb (eqb v1 v1') (is12BitImmediate l1)
+                         then SSeq s2 (SOp v3 op v2' (Const l1))
+                         else default
+                   | SLit v1 l1, _ =>
+                       if andb (eqb v1 v1') (is12BitImmediate l1)
+                       then SSeq s2 (SOp v3 op v2' (Const l1))
+                       else default
+                   | _, SLit v2 l2 =>
+                       if andb (eqb v2 v2') (is12BitImmediate l2)
+                       then SSeq s1 (SOp v3 op v1' (Const l2))
+                       else default
+                   | _, _ => default
                    end
-  | _ => s
-  end.
+               | Syntax.bopname.ltu => (* 0 to 12-bits and all 32 bits down by 12 bits  (FIX THIS LATER) *)
+                   match s2 with
+                   | SLit v2 l2 =>
+                       if andb (eqb v2 v2') (is12BitImmediate l2)
+                       then SSeq s1 (SOp v3 op v1' (Const l2))
+                       else default
+                   | _ => default
+                   end
+               | Syntax.bopname.lts =>
+                   match s2 with
+                   | SLit v2 l2 =>
+                       if andb (eqb v2 v2') (is12BitImmediate l2)
+                       then SSeq s1 (SOp v3 op v1' (Const l2))
+                       else default
+                   | _ => default
+                   end
+               | Syntax.bopname.srs
+               | Syntax.bopname.slu
+               | Syntax.bopname.sru =>
+                   match s2 with
+                   | SLit v2 l2 =>
+                       if andb (eqb v2 v2') (is5BitImmediate l2)
+                       then SSeq s1 (SOp v3 op v1' (Const l2))
+                       else default
+                   | _ => default
+                   end
+               | Syntax.bopname.sub =>
+                   match s2 with
+                   | SLit v2 l2 =>
+                       if andb (eqb v2 v2') (is12BitImmediate (-l2))
+                       then SSeq s1 (SOp v3 Syntax.bopname.add v1' (Const (-l2)))
+                       else default
+                   | _ => default
+                   end
+               | _ => default
+               end
+           | _, _ =>  default
+           end
+    | SStackalloc v1 sz1 s => SStackalloc v1 sz1 (useImmediate s) 
+    | _ => s
+    end.*)
+End WithArgs. 
+
+
+
+
+
+
+Definition useImmOnFlats (t: (list string * list string * stmt string)) : (list string * list string * stmt string)
+  := match t with
+     | (targs, trets, tstmt) => (targs, trets, (useImmediate (fun x => true) (fun x => true)  tstmt))
+     end.
+
+Definition immediateExs := map useImmOnFlats unwrappedFlattenExs.
+Compute immediateExs.
 
