compiler/src/compilerExamples/immediateExample.v
@@ -1,0 +1,216 @@
+Require Import Coq.Lists.List.
+Import ListNotations.
+Require bedrock2Examples.Demos.
+Require Import coqutil.Decidable.
+Require Import compiler.ExprImp.
+Require Import compiler.NameGen.
+Require Import compiler.Pipeline.
+Require Import riscv.Spec.Decode.
+Require Import riscv.Utility.Words32Naive.
+Require Import riscv.Utility.DefaultMemImpl32.
+Require Import riscv.Utility.Monads.
+Require Import compiler.util.Common.
+Require Import coqutil.Decidable.
+Require        riscv.Utility.InstructionNotations.
+Require Import riscv.Platform.MinimalLogging.
+Require Import bedrock2.MetricLogging.
+Require Import riscv.Platform.MetricMinimal.
+Require Import riscv.Utility.Utility.
+Require Import riscv.Utility.Encode.
+Require Import coqutil.Map.SortedList.
+Require Import compiler.MemoryLayout.
+Require Import compiler.StringNameGen.
+Require Import riscv.Utility.InstructionCoercions.
+Require Import riscv.Platform.MetricRiscvMachine.
+Require bedrock2.Hexdump.
+Require Import bedrock2Examples.swap.
+Require Import bedrock2Examples.stackalloc.
+Require Import compilerExamples.SpillingTests.
+
+Open Scope Z_scope.
+Open Scope string_scope.
+Open Scope ilist_scope.
+
+Definition var: Set := Z.
+Definition Reg: Set := Z.
+
+
+Local Existing Instance DefaultRiscvState.
+
+Axiom TODO: forall {T: Type}, T.
+
+Local Instance funpos_env: map.map string Z := SortedListString.map _.
+
+Definition compile_ext_call(posenv: funpos_env)(mypos stackoffset: Z)(s: FlatImp.stmt Z) :=
+  match s with
+  | FlatImp.SInteract _ fname _ =>
+    if string_dec fname "nop" then
+      [[Addi Register0 Register0 0]]
+    else
+      nil
+  | _ => []
+  end.
+
+Notation RiscvMachine := MetricRiscvMachine.
+
+Local Existing Instance coqutil.Map.SortedListString.map.
+Local Existing Instance coqutil.Map.SortedListString.ok.
+
+Definition main_stackalloc :=
+  ("main", ([]: list String.string, []: list String.string,
+     cmd.stackalloc "x" 4 (cmd.stackalloc "y" 4 (cmd.call [] "swap_swap" [expr.var "x"; expr.var "y"])))).
+
+Definition allFuns: list Syntax.func := [swap; swap_swap; main_stackalloc; stacknondet; stackdisj; long1].
+
+(* stack grows from high addreses to low addresses, first stack word will be written to
+   (stack_pastend-8), next stack word to (stack_pastend-16) etc *)
+Definition stack_pastend: Z := 2048.
+
+Lemma f_equal2: forall {A B: Type} {f1 f2: A -> B} {a1 a2: A},
+    f1 = f2 -> a1 = a2 -> f1 a1 = f2 a2.
+Proof. intros. congruence. Qed.
+
+Lemma f_equal3: forall {A B C: Type} {f1 f2: A -> B -> C} {a1 a2: A} {b1 b2: B},
+    f1 = f2 -> a1 = a2 -> b1 = b2 -> f1 a1 b1 = f2 a2 b2.
+Proof. intros. congruence. Qed.
+
+Lemma f_equal3_dep: forall {A B C: Type} {f1 f2: A -> B -> C} {a1 a2: A} {b1 b2: B},
+    f1 = f2 -> a1 = a2 -> b1 = b2 -> f1 a1 b1 = f2 a2 b2.
+Proof. intros. congruence. Qed.
+
+
+Local Instance RV32I_bitwidth: FlatToRiscvCommon.bitwidth_iset 32 RV32I.
+Proof. reflexivity. Qed.
+
+Definition swap_asm: list Instruction.
+  let r := eval cbv in (compile compile_ext_call allFuns) in set (res := r).
+  match goal with
+  | res := Success (?x, _, _) |- _ => exact x
+  end.
+Defined.
+
+Module PrintAssembly.
+  Import riscv.Utility.InstructionNotations.
+  Goal True. let r := eval unfold swap_asm in swap_asm in idtac (* r *). Abort.
+  (*
+  swap_swap:
+     addi    x2, x2, -20   // decrease sp
+     sw      x2, x1, 8     // save ra
+     sw      x2, x3, 0     // save registers modified by swap_swap
+     sw      x2, x4, 4
+     lw      x3, x2, 12    // load args
+     lw      x4, x2, 16
+     sw      x2, x3, -8    // store args for first call to swap
+     sw      x2, x4, -4
+     jal     x1, 36        // first call to swap
+     sw      x2, x3, -8    // store args for second call to swap
+     sw      x2, x4, -4
+     jal     x1, 24        // second call to swap
+     lw      x3, x2, 0     // restore registers modified by swap_swap
+     lw      x4, x2, 4
+     lw      x1, x2, 8     // load ra
+     addi    x2, x2, 20    // increase sp
+     jalr    x0, x1, 0     // return
+
+  swap:
+     addi    x2, x2, -28   // decrease sp
+     sw      x2, x1, 16    // save ra
+     sw      x2, x5, 0     // save registers modified by swap
+     sw      x2, x6, 4
+     sw      x2, x3, 8
+     sw      x2, x4, 12
+     lw      x3, x2, 20    // load args
+     lw      x4, x2, 24
+     lw      x5, x4, 0     // body of swap
+     lw      x6, x3, 0
+     sw      x4, x6, 0
+     sw      x3, x5, 0
+     lw      x5, x2, 0     // restore registers modified by swap
+     lw      x6, x2, 4
+     lw      x3, x2, 8
+     lw      x4, x2, 12
+     lw      x1, x2, 16    // restore ra
+     addi    x2, x2, 28    // increase sp
+     jalr    x0, x1, 0     // return
+
+  stacknondet:
+     addi    x2, x2, -56
+     sw      x2, x1, 44
+     sw      x2, x5, 4
+     sw      x2, x6, 8
+     sw      x2, x7, 12
+     sw      x2, x3, 16
+     sw      x2, x8, 20
+     sw      x2, x9, 24
+     sw      x2, x10, 28
+     sw      x2, x11, 32
+     sw      x2, x12, 36
+     sw      x2, x4, 40
+     addi    x5, x2, 0
+     lw      x6, x5, 0
+     addi    x7, x0, 8
+     srl     x3, x6, x7
+     addi    x8, x0, 3
+     add     x9, x3, x8
+     addi    x10, x0, 42
+     sb      x9, x10, 0
+     lw      x11, x5, 0
+     addi    x12, x0, 8
+     srl     x4, x11, x12
+     sw      x2, x3, 48
+     sw      x2, x4, 52
+     lw      x5, x2, 4
+     lw      x6, x2, 8
+     lw      x7, x2, 12
+     lw      x3, x2, 16
+     lw      x8, x2, 20
+     lw      x9, x2, 24
+     lw      x10, x2, 28
+     lw      x11, x2, 32
+     lw      x12, x2, 36
+     lw      x4, x2, 40
+     lw      x1, x2, 44
+     addi    x2, x2, 56
+     jalr    x0, x1, 0
+
+  stackdisj:
+     addi    x2, x2, -28
+     sw      x2, x1, 16
+     sw      x2, x3, 8
+     sw      x2, x4, 12
+     addi    x3, x2, 4
+     addi    x4, x2, 0
+     sw      x2, x3, 20
+     sw      x2, x4, 24
+     lw      x3, x2, 8
+     lw      x4, x2, 12
+     lw      x1, x2, 16
+     addi    x2, x2, 28
+     jalr    x0, x1, 0
+
+  main:
+     addi    x2, x2, -20   // decrease sp
+     sw      x2, x1, 16    // save ra
+     sw      x2, x3, 8     // save registers modified by main
+     sw      x2, x4, 12
+     addi    x3, x2, 4     // first stackalloc invocation returns sp+4
+     addi    x4, x2, 0     // second stackalloc invocation returns sp
+     sw      x2, x3, -8    // store args for call to swap_swap
+     sw      x2, x4, -4
+     jal     x1, -380      // call swap_swap
+     lw      x3, x2, 8     // restore registers modified by main
+     lw      x4, x2, 12
+     lw      x1, x2, 16    // restore ra
+     addi    x2, x2, 20    // increase sp
+     jalr    x0, x1, 0     // return
+  *)
+End PrintAssembly.
+
+Definition swap_as_bytes: list Byte.byte := instrencode swap_asm.
+
+Module PrintBytes.
+  Import bedrock2.Hexdump.
+  Local Open Scope hexdump_scope.
+  Set Printing Width 100.
+  Goal True. let x := eval cbv in swap_as_bytes in idtac (* x *). Abort.
+End PrintBytes.
